git-svn-id: svn://scm.gforge.inria.fr/svn/cfml@121 ba02c806-7d2b-4818-9a48-35b22e6bdc79

vacid/sparse_array_proof.v
@@ -12,7 +12,9 @@ Definition repr_valid n Back Val T :=
       then T\[i] = Val\[i] 
       else T\[i] = 0.
 
-Definition Sarray (T:array int) l :=
+(* Definition of "l ~> Sarray T" *)
+
+Definition Sarray (T:array int) (l:loc) : heap -> Prop :=
   hexists n (val idx back : loc) (Val Idx Back : array int),
     l ~> sparse_array_of n val idx back 
   * val ~> Array Pure Val
@@ -20,25 +22,37 @@ Definition Sarray (T:array int) l :=
   * back ~> Array Pure Back
   * [ size Val = L /\ 
       size Idx = L /\
-      size Back = L ]
-  * [ idx_back_coherent n Back Idx ]
-  * [ repr_valid n Back Val T ].
+      size Back = L /\
+      idx_back_coherent n Back Idx /\
+      repr_valid n Back Val T ].
 
 
 Lemma used_cell_test_correct : forall n Back Idx i, 
   index L i -> idx_back_coherent n Back Idx ->
   (back_pointed n Back i) <-> (index n (Idx\[i]) /\ Back\[Idx\[i]] = i).
 
-
 Lemma create_spec :
   Spec create size |R>> (0 <= size <= L) -> 
-    R [] (_~> Sarray (Array.make (abs size) 0)).
+    R [] (fun l => l ~> Sarray (CoqArray.make size default)).
+  
+  spec_1 create (fun size R => ...).
 
 Lemma get_spec :
   Spec get i l |R>> forall T, index T i -> 
+    R (l ~> Sarray T) (fun v => l ~> Sarray T * [v = T\[i]]).
+    
     keep R (l ~> Sarray T) (= T\[i]).
 
 Lemma set_spec :
   Spec set i v l |R>> forall T, index T i ->
     R (l ~> Sarray T) (# l ~> Sarray (T\[i:=v])
 
+
+
+(* ---------
+invariant:
+   0 <= n < size <= maxlen
+   forall i, 0 <= i < n -> 0 <= back[i] < sz /\ idx[back[i]] = i
+*)
+
+  (*back_pointed: index n (Idx\[i]) /\ Back\[Idx\[i]] = i *)
