vacid/binary_heap_proof.v
@@ -1,0 +1,27 @@
+Spec empty () |R>> 
+  R [] (_~> Heap \{})
+
+Spec insert l v |R>> forall E, 
+  R (l ~> Heap E) (# l ~> Heap (E \u v))
+
+Spec extract l |R>> forall E, 
+  R (l ~> Heap E) (fun v => 
+    hexists E', l ~> Heap E' * [removed_min E E' V])
+
+Definition removed_min E E' V :=
+  E = E' \u V /\ (forall_ V' \in E, V <= V').
+
+-----
+
+Spec empty () |R>> 
+  forall T, R [] (_~> Heap T \{})
+
+
+Spec insert l v |R>> forall T E V, 
+  R (l ~> Heap T E * T V v) (# l ~> Heap T (E \u V))
+
+Spec extract l |R>> forall T E, 
+  R (l ~> Heap T E) (fun v => 
+    hexists E' V, l ~> Heap T E' * T V v * [removed_min E E' V])
+
+-------
