vacid/rb_tree_proof.v
@@ -1,0 +1,36 @@
+
+Spec empty () |R>> 
+  R [] (_~> Tree \{})
+
+Spec get l k |R>> forall M, 
+  R (l ~> Tree M) (fun o => l ~> Tree M * [o = map_get_option M k])
+
+  keep R (l ~> Tree M) (= map_get_option M k)
+
+Spec set l k v |R>> forall M,
+  R (l ~> Tree M) (# l ~> Tree (M \u \[k := v]))
+
+Spec rem l k |R>> forall M,
+  R (l ~> Tree M) (l ~> Tree (M \rem l))
+
+
+l ~> Tree M  
+Tree M l
+exists n, TreeRec n Black M l
+
+TreeRec n c M l : hprop = hexists o,
+  l ~> o *
+  match o with
+  | None => [n = 1 /\ c = Black]
+  | Some (k,v,l1,l2,c') =>
+     hexists c1 c2 M1 M2 n',
+       l1 ~> TreeRec n' c1 M1 
+     * l2 ~> TreeRec n' c2 M2
+     * [ c' = c
+      /\ n' = (if c = Black then n-1 else n)
+      /\ (c = Red -> c1 = Black /\ c2 = Black)
+      /\ foreach M1 (fun k' v' => k' < k)
+      /\ foreach M2 (fun k' v' => k' > k)
+      /\ M = M1 \u M2 \u \[k:=v]
+      ]
+
